Java/src/Java/Func/Reify.v
@@ -1,5 +1,5 @@
 Require Import MirrorCore.Reify.Reify.
-Require Import MirrorCore.Reify.ReifyView.
+Require Import MirrorCore.Reify.ReifyView. 
 Require Import MirrorCore.Lambda.Expr.
 Require Import MirrorCore.syms.SymOneOf.
 Require Import MirrorCore.Lib.ListView.
@@ -40,6 +40,13 @@ Require Import ChargeCore.Logics.Later.
 Require Import ExtLib.Structures.Applicative.
 Require Import MirrorCore.Lib.NatView.
 
+Reify Declare Typed Table term_table : BinNums.positive => typ.
+
+Local Instance Applicative_Fun A : Applicative (RFun A) :=
+{ pure := fun _ x _ => x
+; ap := fun _ _ f x y => (f y) (x y)
+}.
+
 Global Instance Reify_typ : Reify typ :=
   Reify_typ typ (reify_base_typ typ ::
                  reify_list_typ typ ::
@@ -48,26 +55,112 @@ Global Instance Reify_typ : Reify typ :=
                  reify_java_typ typ :: nil).
 
 Global Instance Reify_java : Reify (expr typ func) :=
-  Reify_func typ func (reify_nat typ func :: 
-(*                       reify_bool typ func ::
-                       reify_string typ func ::
-Removing the comments for these two makes the syntax declaration for exprs fail, but 
-we get no universe inconsistency.
-*)
-                       reify_eq typ func ::
-                       reify_applicative typ func (Fun (String.string -> val)) ::
-                       reify_list typ func :: 
-                       reify_listOp typ func :: 
-                       reify_prod typ func ::
-          	       reify_ilogic typ func :: 
-                       reify_bilogic typ func ::
-                       reify_embed typ func ::
-                       reify_subst typ func String.string val :: nil).
-
-Set Printing Universes.
+  Reify_func typ func term_table (reify_java_func ::
+                                  reify_nat typ func ::
+                                  reify_bool typ func ::
+                                  reify_string typ func :: 
+                                  reify_eq typ func ::
+                                  reify_applicative typ func (RFun (RFun String.string val)) ::
+                                  reify_list typ func :: 
+                                  reify_listOp typ func :: 
+                                  reify_prod typ func ::
+          	                  reify_ilogic typ func :: 
+          	                  reify_plogic typ func :: 
+                                  reify_bilogic typ func ::
+                                  reify_embed typ func ::
+                                  reify_subst typ func String.string val :: nil).
 
 Reify Declare Syntax reify_typ := reify_scheme@{Set} typ.
-Reify Declare Syntax reify_java := reify_scheme (expr typ func).
+Reify Declare Syntax reify_java := reify_scheme@{Set} (expr typ func).
+
+Let elem_ctor : forall x : typ, typD x -> @SymEnv.function _ _ :=
+  @SymEnv.F _ _.
+
+Ltac reify_java e :=
+  let k fs e :=
+      pose e in
+  reify_expr reify_java k
+             [[ (fun (y : @mk_dvar_map _ _ _ _ term_table elem_ctor) => True) ]]
+             [[ e ]].
+
+Ltac reify_typ e :=
+  let k fs e :=
+      pose e in
+  reify_expr reify_typ k
+             [[ (fun (y : @mk_dvar_map _ _ _ _ term_table elem_ctor) => True) ]]
+             [[ e ]].
+
+Goal (forall (Pr : Program) (C : class) (v : val) (x f : String.string) (fields : list field) (ex : @Open.expr Lang.var val), True).
+  intros Pr C v x f fields ex.
+  reify_java 5.
+  reify_java (typeof C v).
+  reify_java (field_lookup).
+  reify_java (5::4::3::@nil nat).
+  reify_java (field_lookup Pr C fields).
+  reify_java True.
+  reify_java False.
+  reify_java (True \/ False).
+  reify_java (True /\ False).
+  reify_java (False -> True).
+  reify_java (5 = 5).
+  reify_java (exists x, x = 5).
+  reify_java (forall x, x = 5).
+
+  reify_java (pure (T := RFun (RFun String.string val)) pointsto).
+
+  reify_java (fun a b c => pointsto a b c).
+
+
+  pose (E_val (vint 3)) as d.
+
+  reify_java (pure (T := RFun (RFun String.string val)) (vbool true)).
+
+  reify_java (forall x : nat, x = x).
+  reify_java (exists x : Lang.stack, True).
+  reify_java (ap (T := RFun (RFun String.string val)) (pure (T := RFun (RFun String.string val)) (@eq val)) (eval d)).
+
+  reify_java ((ap (ap (T := Fun Lang.stack) (pure (T := Fun Lang.stack) (@eq val)) (eval d)) (pure (vbool true)))).
+
+  generalize String.EmptyString. intro c.
+  reify_java (cread c c c).
+
+   reify_java (ltrue |-- {[ ltrue ]} cread c c c {[ ltrue ]}).
+
+  reify_java cskip.
+
+  reify_java (forall P, P /\ P).
+
+  reify_java (forall x : nat, x = x).
+  reify_java (exists x : nat, x = x).
+
+  reify_java (@subst1 Lang.var val _).
+  reify_java (cseq cskip cskip).
+
+  reify_java (@map nat nat).
+  reify_java (ILogic.lentails True True).
+
+  reify_java ((True -> False) -> True).
+  reify_java (forall P Q, P /\ Q).
+
+  reify_java (forall P : sasn, ILogic.lentails ILogic.ltrue P).
+  reify_java (forall (G : spec) (P Q : sasn), ILogic.lentails G (triple P Q cskip)).
+  generalize (String.EmptyString : String.string).
+  intro y.
+
+  reify_java (stack_get (A := Lang.var) (val := val)).
+  reify_java (@stack_get Lang.var val y).
+
+  reify_java (stack_get (val := val) y).
+
+  reify_java (y = y).
+
+  reify_java (@ltrue sasn _).
+
+  exact I.
+
+Defined.
+
+
 
 Ltac reify trm :=
   let t := fresh "t" in
